src/Prototype/LanguageFacts.v
@@ -1,0 +1,43 @@
+Require Import Bool List String Peano_dec.
+Require Import FunctionalExtensionality.
+Require Import Tactics FMap Language.
+
+Section Facts.
+  Variable MsgT: Type.
+  Hypothesis (msgT_dec: forall m1 m2: MsgT, {m1 = m2} + {m1 <> m2}).
+  Variable ValT: Type.
+  Hypothesis (valT_dec: forall m1 m2: ValT, {m1 = m2} + {m1 <> m2}).
+  Variable StateT: Type.
+
+  Local Notation Msg := (Msg MsgT ValT).
+  Local Notation Label := (Label MsgT ValT).
+  Local Notation step_sys := (step_sys msgT_dec valT_dec).
+  Local Notation System := (System MsgT ValT StateT).
+
+  Definition ValidLabel (l: Label) :=
+    match lbl_hdl l with
+    | Some hdl => lbl_ins l = nil /\ ValidOuts (msgTo (msg_id hdl)) (lbl_outs l)
+    | None => lbl_outs l = nil
+    end.
+
+  Lemma step_sys_validLabel:
+    forall (sys: System) st1 l st2, step_sys sys st1 l st2 -> ValidLabel l.
+  Proof.
+    induction 1; simpl; intros.
+    - inv H3.
+      + split; [reflexivity|].
+        simpl; rewrite H6; assumption.
+      + cbv; auto.
+    - unfold ValidLabel in *.
+      destruct lbl1 as [ins1 hdl1 outs1], lbl2 as [ins2 hdl2 outs2]; simpl in *.
+      destruct hdl1 as [hdl1|], hdl2 as [hdl2|].
+      + simpl; reflexivity.
+      + simpl; split; [reflexivity|].
+        admit.
+      + simpl; split; [reflexivity|].
+        admit.
+      + simpl; reflexivity.
+  Admitted.
+
+End Facts.
+
